src/phase2/flexible_completion.lean
@@ -71,6 +71,15 @@ begin
   exact this hL,
 end
 
+lemma flexible_completion_symm_smul_flexible (hπ : π.free α A) (L : litter) (hL : flexible α L A) :
+  flexible α ((flexible_completion α π A).symm • L) A :=
+begin
+  have := local_perm.map_domain (flexible_completion α π A).symm.litter_perm,
+  rw [symm_litter_perm, local_perm.symm_domain,
+    flexible_completion_litter_perm_domain_free α π A hπ] at this,
+  exact this hL,
+end
+
 end near_litter_approx
 
 end con_nf
